Progress

theories/Dot/misc_unused/dot_lty.v
@@ -1,12 +1,8 @@
 From iris.proofmode Require Import tactics.
-From D Require Export iris_prelude.
+From D Require Export iris_prelude proper.
 From D Require Import lty ty_interp_subst_lemmas pty_interp_subst_lemmas.
 From D.Dot Require Import syn syn.path_repl dlang_inst path_wp lr_syn_aux.
 From D.pure_program_logic Require Import lifting.
-
-Notation "'λI' x .. y , t" := (fun x => .. (fun y => t%I) ..)
-  (at level 200, x binder, y binder, right associativity, only parsing,
-  format "'[  ' '[  ' 'λI'  x  ..  y ']' ,  '/' t ']'") : function_scope.
 
 Implicit Types (Σ : gFunctors).
 Implicit Types
@@ -23,7 +19,6 @@ Import persistent_ty_interp_lemmas.
 
 (** Override notations to specify scope. *)
 Notation "p⟦ T ⟧" := (pty_interp T%ty).
-(* Notation "p⟦ Γ ⟧*" := (pty_interp <$> Γ). *)
 Notation "p⟦ Γ ⟧*" := (fmap (M := list) pty_interp Γ).
 
 Definition dslty Σ := env -> iPPred dms Σ.
@@ -35,8 +30,8 @@ Record dlty Σ := Dlty {
   dlty_car :> env -> iPPred dm Σ;
 }.
 Global Arguments Dlty {_} _%I _.
-Global Arguments dlty_label {_} _ /.
-Global Arguments dlty_car {_} !_ _ /.
+Global Arguments dlty_label {_} !_ /.
+Global Arguments dlty_car {_} !_ /.
 
 (* Forces inserting coercions to -d>. *)
 Notation dApp := (dlty_car : dlty _ → _ -d> _).
@@ -62,23 +57,6 @@ Section defs.
   Definition lift_dlty (φ : dlty Σ) l : envPred dm Σ :=
     λI ρ d, ⌜ dlty_label φ = l ⌝ ∧ φ ρ d.
 
-  (* Definition sdtp Γ TD l d : iProp Σ :=
-    (⌜ l = dlty_label TD ⌝ ∧
-      □∀ ρ, s⟦Γ⟧* ρ → TD ρ d.|[ρ])%I. *)
-  Definition sdtp Γ (φ : dlty Σ) l d : iProp Σ :=
-    □∀ ρ, ⌜path_includes (pv (ids 0)) ρ [(l, d)] ⌝ → s⟦Γ⟧* ρ → lift_dlty φ l ρ d.|[ρ].
-  Global Arguments sdtp /.
-
-  (** Multi-definition typing *)
-  Definition sdstp Γ (T : dslty Σ) ds : iProp Σ :=
-    ⌜wf_ds ds⌝ ∧ □∀ ρ, ⌜path_includes (pv (ids 0)) ρ ds ⌝ → s⟦Γ⟧* ρ → T ρ ds.|[ρ].
-  Global Arguments sdstp /.
-
-  Definition sptp Γ T p i: iProp Σ :=
-    □∀ ρ, s⟦Γ⟧* ρ -∗
-      ▷^i path_wp (p.|[ρ]) (λ v, oClose T ρ v).
-  Global Arguments sptp /.
-
   Context {i : nat}.
   Implicit Types (φ : hoEnvD Σ i) (τ : olty Σ i).
   (*
@@ -93,6 +71,23 @@ Section defs.
   Definition dm_to_type d i (ψ : hoD Σ i) : iProp Σ :=
     (∃ s σ, ⌜ d = dtysem σ s ⌝ ∧ s ↗n[ σ , i ] ψ)%I.
 End defs.
+
+(* Definition sdtp Γ TD l d : iProp Σ :=
+  (⌜ l = dlty_label TD ⌝ ∧
+    □∀ ρ, s⟦Γ⟧* ρ → TD ρ d.|[ρ])%I. *)
+Definition sdtp `{HdotG: dlangG Σ} Γ (φ : dltyO Σ) l d : iProp Σ :=
+  □∀ ρ, ⌜path_includes (pv (ids 0)) ρ [(l, d)] ⌝ → s⟦Γ⟧* ρ → lift_dlty φ l ρ d.|[ρ].
+Global Arguments sdtp /.
+
+(** Multi-definition typing *)
+Definition sdstp `{HdotG: dlangG Σ} Γ (T : dsltyO Σ) ds : iProp Σ :=
+  ⌜wf_ds ds⌝ ∧ □∀ ρ, ⌜path_includes (pv (ids 0)) ρ ds ⌝ → s⟦Γ⟧* ρ → T ρ ds.|[ρ].
+Global Arguments sdstp /.
+
+Definition sptp `{HdotG: dlangG Σ} Γ (T : oltyO Σ 0) p i: iProp Σ :=
+  □∀ ρ, s⟦Γ⟧* ρ -∗
+    ▷^i path_wp (p.|[ρ]) (λ v, oClose T ρ v).
+Global Arguments sptp /.
 
 Notation "Γ s⊨ {  l := d  } : T" := (sdtp Γ T l d) (at level 64, d, l, T at next level).
 Notation "Γ s⊨p p : τ , i" := (sptp Γ τ p i) (at level 74, p, τ, i at next level).
@@ -128,7 +123,7 @@ End dm_to_type.
 Section SemTypes.
   Context `{HdotG: dlangG Σ}.
 
-  Implicit Types (τ : olty Σ 0).
+  Implicit Types (τ : oltyO Σ 0).
    (* (ψ : vl -d> iPropO Σ) (φ : envD Σ)  *)
 
   Program Definition lift_dinterp_vl (TD : dlty Σ): olty Σ 0 :=
@@ -173,7 +168,7 @@ Section SemTypes.
      typechecking this example needs to establish x.T <: TNat having in context
      only x: {T <: TNat; U <: x.T -> TNat}.
    *)
-  Definition oForall τ1 τ2 := olty0
+  Definition oAll τ1 τ2 := olty0
     (λI ρ v,
     (∃ t, ⌜ v = vabs t ⌝ ∧
      □ ∀ w, ▷ τ1 vnil ρ w → ▷ interp_expr τ2 (w .: ρ) t.|[w/])).
@@ -192,7 +187,7 @@ Section SemTypes.
     | TPrim b => oPrim b
     | TTop => oTop
     | TBot => oBot
-    | TAll T1 T2 => oForall p⟦ T1 ⟧ p⟦ T2 ⟧
+    | TAll T1 T2 => oAll p⟦ T1 ⟧ p⟦ T2 ⟧
     | TMu T => oMu p⟦ T ⟧
     | TSel p l => oTSel p l
     | TSing p => oPSing p
@@ -221,7 +216,7 @@ Section SemTypes.
   Program Definition defs_interp_and (interp1 interp2 : dslty Σ) : dslty Σ :=
     Dslty (λI ρ ds, interp1 ρ ds ∧ interp2 ρ ds).
 
-  Definition lift_dinterp_dms (T : dlty Σ) : dslty Σ := Dslty (λI ρ ds,
+  Definition lift_dinterp_dms (T : dltyO Σ) : dsltyO Σ := Dslty (λI ρ ds,
     ∃ l d, ⌜ dms_lookup l ds = Some d ⌝ ∧ lift_dlty T l ρ d).
 
   Fixpoint defs_interp T : dslty Σ :=
@@ -301,7 +296,8 @@ Section SampleTypingLemmas.
     iIntros "H"; iSplit; first done; iExists p. by auto.
   Qed.
 
-  Lemma Sub_Sel Γ L U va l i:
+  Context {Γ : sCtx Σ}.
+  Lemma sSub_Sel L U va l i:
     Γ s⊨ tv va : oTTMem l L U, i -∗
     Γ s⊨ oLater L, i <: oTSel (pv va) l, i.
   Proof.
@@ -312,7 +308,7 @@ Section SampleTypingLemmas.
     iExists ψ, d; repeat iSplit => //. by iApply "HLψ".
   Qed.
 
-  Lemma Sel_Sub Γ L U va l i:
+  Lemma sSel_Sub L U va l i:
     Γ s⊨ tv va : oTTMem l L U, i -∗
     Γ s⊨ oTSel (pv va) l, i <: oLater U, i.
   Proof.
@@ -325,7 +321,7 @@ Section SampleTypingLemmas.
     iApply "HψU" => //. iNext. by iRewrite "Hag".
   Qed.
 
-  Lemma D_Typ_Abs Γ T L U s σ l:
+  Lemma sD_Typ_Abs T L U s σ l:
     Γ s⊨ oLater T, 0 <: oLater U, 0 -∗
     Γ s⊨ oLater L, 0 <: oLater T, 0 -∗
     s ↝[ σ ] T -∗
@@ -340,10 +336,90 @@ Section SampleTypingLemmas.
     - iApply "HTU" => //. by iApply Hγφ.
   Qed.
 
-  Lemma D_Typ Γ (τ : olty Σ 0) s σ l:
+  Lemma sD_Typ (τ : olty Σ 0) s σ l:
     s ↝[ σ ] τ -∗
     Γ s⊨ { l := dtysem σ s } : oDTMem l τ τ.
-  Proof. iIntros "#Hs"; iApply D_Typ_Abs; by [| iIntros "!> **"]. Qed.
+  Proof. iIntros "#Hs"; iApply sD_Typ_Abs; by [| iIntros "!> **"]. Qed.
+
+  (*
+     Γ, z: T₁ᶻ ⊨ T₁ᶻ <: T₂ᶻ
+     ----------------------------------------------- (<:-μ-X)
+     Γ ⊨ μ (x: T₁ˣ) <: μ(x: T₂ˣ)
+  *)
+  (* Notation "◁ n T ▷" := (iterate TLater n T). *)
+  Lemma sSub_Mu_X T1 T2 i j:
+    iterate oLater i T1 :: Γ s⊨ T1, i <: T2, j -∗
+    Γ s⊨ oMu T1, i <: oMu T2, j.
+  Proof.
+    iIntros "/= #Hstp !>" (vs v) "#Hg #HT1".
+    iApply ("Hstp" $! (v .: vs) v with "[# $Hg] [#//]").
+    by rewrite iterate_TLater_later.
+  Qed.
+
+  Lemma sSub_Mu_A T i: Γ s⊨ oMu (shift T), i <: T, i.
+  Proof. iIntros "!> **". by rewrite interp_TMu_ren. Qed.
+
+  Lemma sSub_Mu_B T i: Γ s⊨ T, i <: oMu (shift T), i.
+  Proof. iIntros "!> **". by rewrite interp_TMu_ren. Qed.
+
+  (*
+     Γ ⊨ z: Tᶻ
+     =============================================== (T-Rec-I/T-Rec-E)
+     Γ ⊨ z: mu(x: Tˣ)
+   *)
+  Lemma sTMu_equiv T v: (Γ s⊨ tv v : oMu T) ≡ (Γ s⊨ tv v : T.|[v/]).
+  Proof.
+    iSplit; iIntros "#Htp !>" (vs) "#Hg !> /=";
+    iDestruct (wp_value_inv' with "(Htp Hg)") as "{Htp} Hgoal";
+    rewrite -wp_value/= (hoEnvD_subst_one _ v (v.[vs])); done.
+  Qed.
+
+  (*
+     Γ ⊨ z: Tᶻ
+     =============================================== (T-Rec-I/T-Rec-E)
+     Γ ⊨ z: mu(x: Tˣ)
+   *)
+  Lemma sTMu_I T v: Γ s⊨ tv v : T.|[v/] -∗ Γ s⊨ tv v : oMu T.
+  Proof. by rewrite sTMu_equiv. Qed.
+
+  Lemma sTMu_E T v: Γ s⊨ tv v : oMu T -∗ Γ s⊨ tv v : T.|[v/].
+  Proof. by rewrite sTMu_equiv. Qed.
+
+  Lemma sT_Forall_E e1 e2 T1 T2:
+    Γ s⊨ e1 : oAll T1 (shift T2) -∗
+    Γ s⊨ e2 : T1 -∗
+    (*────────────────────────────────────────────────────────────*)
+    Γ s⊨ tapp e1 e2 : T2.
+  Proof.
+    iIntros "/= #He1 #Hv2 !>" (vs) "#HG !>".
+    smart_wp_bind (AppLCtx (e2.|[_])) v "#Hr" ("He1" with "[]").
+    smart_wp_bind (AppRCtx v) w "#Hw" ("Hv2" with "[]").
+    iDestruct "Hr" as (t ->) "#Hv".
+    rewrite -wp_pure_step_later // -wp_mono /=; first by iSpecialize ("Hv" with "Hw"); iNext.
+    iIntros (v); by rewrite /= (hoEnvD_weaken_one T2 _ _ _).
+  Qed.
+
+  Lemma sT_Forall_Ex e1 v2 T1 T2:
+    Γ s⊨ e1: oAll T1 T2 -∗
+    Γ s⊨ tv v2 : T1 -∗
+    (*────────────────────────────────────────────────────────────*)
+    Γ s⊨ tapp e1 (tv v2) : T2.|[v2/].
+  Proof.
+    iIntros "/= #He1 #Hv2Arg !> * #HG !>".
+    smart_wp_bind (AppLCtx (tv v2.[_])) v "#Hr {He1}" ("He1" with "[#//]").
+    iDestruct "Hr" as (t ->) "#HvFun".
+    rewrite -wp_pure_step_later; last done.
+    iSpecialize ("HvFun" with "[#]"). {
+      rewrite -wp_value_inv'. by iApply ("Hv2Arg" with "[]").
+    }
+    iNext. iApply wp_wand.
+    - iApply "HvFun".
+    - iIntros (v) "{HG HvFun Hv2Arg} H".
+      rewrite /= (hoEnvD_subst_one T2 v2 v) //.
+  Qed.
+
+  Lemma pty_interp_subst (T : ty) σ : p⟦ T.|[σ] ⟧ ≡ (p⟦ T ⟧).|[σ].
+  Proof. intros ???; apply interp_subst_compose_ind. Qed.
 End SampleTypingLemmas.
 
 Module ty_compat.
@@ -351,8 +427,16 @@ Module ty_compat.
 Include TyInterpLemmas VlSorts dlang_inst.
 Notation "⟦ T ⟧" := (ty_interp T%ty).
 
+Ltac solve_proper_ho_equiv_core tac :=
+  solve [repeat intro; cbn; repeat tac (); cbn in *;
+  repeat match goal with H : _ ≡ _|- _ => apply H || rewrite H // end].
+Ltac solve_proper_ho_equiv :=
+  solve_proper_prepare; properness => //;
+  solve_proper_ho_equiv_core ltac:(fun _ => idtac).
+
 Section defs.
   Context `{HdotG: dlangG Σ}.
+
   (* Wrap this into ty_interp to reuse lemmas. *)
   Global Instance pto_ty_interp : TyInterp ty Σ := flip pty_interp vnil.
   Global Instance interp_persistent T ρ v : Persistent (⟦ T ⟧ ρ v) := _.
@@ -371,65 +455,104 @@ Section defs.
   (* Lemma swap0 T σ args ρ v : p⟦ T.|[σ] ⟧ args ρ v ≡ (p⟦ T ⟧).|[σ] args ρ v.
   Proof. apply persistent_ty_interp_lemmas.interp_subst_compose_ind. Qed. *)
 
-  Lemma pty_interp_subst T σ : p⟦ T.|[σ] ⟧ ≡ (p⟦ T ⟧).|[σ].
-  Proof. intros ???; apply persistent_ty_interp_lemmas.interp_subst_compose_ind. Qed.
-
-  (* XXX drop *)
-Section flip_proper.
-Context `{R : relation A} `{S : relation B} `{T : relation C} `{U : relation D} `{V : relation E}.
-Global Instance flip_proper_2 `(!Proper (R ==> S) f) :
-  Proper (flip R ==> flip S) f.
-Proof. solve_proper. Qed.
-Global Instance flip_proper_3 `(!Proper (R ==> S ==> T) f) :
-  Proper (flip R ==> flip S ==> flip T) f.
-Proof. solve_proper. Qed.
-Global Instance flip_proper_4 `(!Proper (R ==> S ==> T ==> U) f) :
-  Proper (flip R ==> flip S ==> flip T ==> flip U) f.
-Proof. solve_proper. Qed.
-Global Instance flip_proper_5 `(!Proper (R ==> S ==> T ==> U ==> V) f) :
-  Proper (flip R ==> flip S ==> flip T ==> flip U ==> flip V) f.
-Proof. solve_proper. Qed.
-End flip_proper.
-
-Ltac properness :=
-repeat match goal with
-| |- (∃ _: _, _)%I ≡ (∃ _: _, _)%I => apply bi.exist_proper =>?
-| |- (∀ _: _, _)%I ≡ (∀ _: _, _)%I => apply bi.forall_proper =>?
-| |- (_ ∧ _)%I ≡ (_ ∧ _)%I => apply bi.and_proper
-| |- (_ ∨ _)%I ≡ (_ ∨ _)%I => apply bi.or_proper
-| |- (_ → _)%I ≡ (_ → _)%I => apply bi.impl_proper
-| |- (_ -∗ _)%I ≡ (_ -∗ _)%I => apply bi.wand_proper
-| |- (WP _ {{ _ }})%I ≡ (WP _ {{ _ }})%I => apply wp_proper =>?
-| |- (▷ _)%I ≡ (▷ _)%I => apply bi.later_proper
-| |- (▷^_ _)%I ≡ (▷^_ _)%I => apply bi.laterN_proper
-| |- (□ _)%I ≡ (□ _)%I => apply bi.intuitionistically_proper
-| |- (_ ∗ _)%I ≡ (_ ∗ _)%I => apply bi.sep_proper
-(* | |- (inv _ _)%I ≡ (inv _ _)%I => apply (contractive_proper _) *)
-end.
-
-  Global Instance Proper_setp Γ : Proper ((≡) ==> (=) ==> (≡)) (setp Γ).
-  Proof. intros ?? Heq ???; simplify_eq/=. properness; [done|apply Heq]. Qed.
-  Global Instance Proper_setp_flip Γ : Proper (flip (≡) ==> flip (=) ==> flip (≡)) (setp Γ).
-  Proof. apply: flip_proper_3. Qed.
-  Global Instance Proper_sstpi Γ : Proper ((≡) ==> (≡) ==> (=) ==> (=) ==> (≡)) (sstpi (Σ := Σ) Γ).
+  Global Instance Proper_env_oltyped : Proper ((≡) ==> (=) ==> (≡)) (env_oltyped (Σ := Σ)).
   Proof.
-    intros ?? H1 ?? H2 ?** ?**; simplify_eq/=.
-    properness; [done|apply H1|apply H2].
+    move => + + /equiv_Forall2 + + _ <-.
+    elim => [|T1 G1 IHG1] [|T2 G2] /=; [done|inversion 1..|] =>
+      /(Forall2_cons_inv _ _ _ _) [HT HG] ρ; f_equiv; [apply IHG1, HG|apply HT].
   Qed.
-  Global Instance Proper_sstpi_flip Γ : Proper ((≡) --> (≡) --> (=) --> (=) --> flip (≡)) (sstpi (Σ := Σ) Γ).
-  Proof. apply: flip_proper_5. Qed.
+
+  Global Instance Proper_sstpi :
+    Proper ((≡) ==> (≡) ==> (≡) ==> (=) ==> (=) ==> (≡)) (sstpi (Σ := Σ)).
+  Proof.
+    solve_proper_ho_equiv.
+    (* intros ?? HG ?? H1 ?? H2 ?** ?**; simplify_eq/=.
+    properness; [by rewrite HG|apply H1|apply H2]. *)
+  Qed.
+  Global Instance Proper_sstpi_flip :
+    Proper ((≡) --> (≡) --> (≡) --> (=) --> (=) --> flip (≡)) (sstpi (Σ := Σ)).
+  Proof. apply: flip_proper_6. Qed.
+
+
+  Global Instance Proper_setp : Proper ((≡) ==> (≡) ==> (=) ==> (≡)) setp.
+  Proof.
+    solve_proper_ho_equiv.
+    (* intros ?? HG ?? HT ???; simplify_eq/=. by properness; [rewrite HG|apply HT]. *)
+  Qed.
+  Global Instance Proper_setp_flip :
+    Proper (flip (≡) ==> flip (≡) ==> flip (=) ==> flip (≡)) setp.
+  Proof. apply: flip_proper_4. Qed.
+
+  Global Instance: Proper ((≡) ==> (=) ==> (=) ==> (=) ==> (≡)) (lift_dlty (Σ := Σ)).
+  Proof.
+    rewrite /lift_dlty => -[l1 P1] [l2 P2] [/= Heq ?] ??? ??? ???; simplify_eq.
+    solve_proper_ho_equiv.
+    (* properness; [done|apply Heq]. *)
+  Qed.
+
+  Global Instance Proper_sdtp Γ : Proper ((≡) ==> (=) ==> (=) ==> (≡)) (sdtp Γ).
+  Proof.
+    solve_proper_ho_equiv.
+    (* intros ?? Heq ??? ???; simplify_eq/=. by properness; [done..|rewrite Heq]. *)
+  Qed.
+  Global Instance Proper_sdtp_flip Γ : Proper (flip (≡) ==> flip (=) ==> flip (=) ==> flip (≡)) (sdtp (Σ := Σ) Γ).
+  Proof. apply: flip_proper_4. Qed.
+
+  Global Instance Proper_oAll : Proper ((≡) ==> (≡) ==> (≡)) oAll.
+  Proof. solve_proper_ho_equiv. Qed.
 
   Lemma T_Var' Γ x τ
     (Hx : Γ !! x = Some τ):
     (*──────────────────────*)
     Γ ⊨ of_val (ids x) : shiftN x τ.
   Proof.
-    rewrite /ietp pty_interp_subst. apply T_Var.
+    rewrite /ietp (pty_interp_subst τ (ren (+x))). apply T_Var.
     by rewrite list_lookup_fmap Hx.
   Qed.
 
-  (* Lemma setp_wand Γ e τ1 τ2 : Γ s⊨ e : τ1 -∗ ⌜ τ1 ≡ τ2 ⌝ → Γ s⊨ e : τ2.
-  Admitted. *)
+  Lemma iterate_TLater_oLater i T:
+    p⟦iterate TLater i T⟧ ≡ iterate oLater i p⟦T⟧.
+  Proof. elim: i => [//|i IHi] ???. by rewrite !iterate_S /= (IHi _ _ _). Qed.
+
+  Lemma Sub_Mu_X Γ T1 T2 i j:
+    iterate TLater i T1 :: Γ ⊨ T1, i <: T2, j -∗
+    Γ ⊨ TMu T1, i <: TMu T2, j.
+  Proof.
+    rewrite /istpi -sSub_Mu_X.
+    by rewrite fmap_cons (iterate_TLater_oLater i T1).
+  Qed.
+  Context {Γ : ctx}.
+
+  Lemma TMu_I T v: Γ ⊨ tv v : T.|[v/] -∗ Γ ⊨ tv v : TMu T.
+  Proof. by rewrite /ietp -sTMu_I pty_interp_subst. Qed.
+
+  Lemma TMu_E T v: Γ ⊨ tv v : TMu T -∗ Γ ⊨ tv v : T.|[v/].
+  Proof. by rewrite /ietp sTMu_E pty_interp_subst. Qed.
+
+  Global Instance: Params (@bi_entails) 1 := {}.
+  Global Instance: Params (@oAll) 2 := {}.
+  (* Moving eq paramaters first would speed things up. *)
+  Global Instance: Params (@setp) 2 := {}.
+
+  Lemma T_Forall_E e1 e2 T1 T2:
+    Γ ⊨ e1 : TAll T1 (shift T2) -∗
+    Γ ⊨ e2 : T1 -∗
+    (*────────────────────────────────────────────────────────────*)
+    Γ ⊨ tapp e1 e2 : T2.
+  Proof.
+    rewrite /ietp -(sT_Forall_E e1 e2).
+    (* apply equiv_entails. *)
+    by rewrite -(pty_interp_subst T2 (ren(+1))).
+    (* do 3 (properness => //=);
+      apply (pty_interp_subst T2 (ren(+1))). *)
+  Qed.
+
+  Lemma T_Forall_Ex e1 v2 T1 T2:
+    Γ ⊨ e1: TAll T1 T2 -∗
+    Γ ⊨ tv v2 : T1 -∗
+    (*────────────────────────────────────────────────────────────*)
+    Γ ⊨ tapp e1 (tv v2) : T2.|[v2/].
+  Proof. rewrite /ietp (sT_Forall_Ex e1 v2). by rewrite (pty_interp_subst T2). Qed.
 End defs.
 
 End ty_compat.
